code/rsapss/Hacl.Spec.Bignum.Convert.fst
@@ -29,6 +29,15 @@ let bn_from_bytes_be len b =
   bn_from_bytes_be_ bnLen tmp
 
 
+val bn_from_bytes_le: len:size_pos{8 * blocks len 8 <= max_size_t} -> lseq uint8 len -> lbignum (blocks len 8)
+let bn_from_bytes_le len b =
+  let bnLen = blocks len 8 in
+  let tmpLen = 8 * bnLen in
+  let tmp = create tmpLen (u8 0) in
+  let tmp = update_sub tmp 0 len b in
+  uints_from_bytes_le tmp
+
+
 val bn_to_bytes_be_f: len:size_nat{8 * len <= max_size_t} -> lbignum len -> i:nat{i < len} -> unit -> unit & lseq uint8 8
 let bn_to_bytes_be_f len b i () =
   (), uint_to_bytes_be b.[len - i - 1]
@@ -48,6 +57,14 @@ let bn_to_bytes_be len b =
   let tmpLen = 8 * bnLen in
   let tmp = bn_to_bytes_be_ bnLen b in
   sub tmp (tmpLen - len) len
+
+
+val bn_to_bytes_le: len:size_pos{8 * blocks len 8 <= max_size_t} -> lbignum (blocks len 8) -> lseq uint8 len
+let bn_to_bytes_le len b =
+  let bnLen = blocks len 8 in
+  let tmpLen = 8 * bnLen in
+  let tmp = uints_to_bytes_le b in
+  sub tmp 0 len
 
 ///
 ///  Lemmas
@@ -80,12 +97,12 @@ let bn_from_bytes_be_is_uints_from_bytes_be_reverse len b =
   eq_intro (bn_from_bytes_be_ len b) (reverse (uints_from_bytes_be b))
 
 
-val bn_v_is_nat_from_intseq_le_lemma: len:size_nat -> b:lseq uint64 len -> Lemma (bn_v b == nat_from_intseq_be (reverse b))
-let rec bn_v_is_nat_from_intseq_le_lemma len b =
+val bn_v_is_nat_from_intseq_be_lemma: len:size_nat -> b:lseq uint64 len -> Lemma (bn_v b == nat_from_intseq_be (reverse b))
+let rec bn_v_is_nat_from_intseq_be_lemma len b =
   if len = 0 then bn_eval0 b
   else begin
     let b1 = slice b 0 (len - 1) in
-    bn_v_is_nat_from_intseq_le_lemma (len - 1) b1;
+    bn_v_is_nat_from_intseq_be_lemma (len - 1) b1;
     assert (bn_v b1 == nat_from_intseq_be (reverse b1));
 
     bn_eval_split_i #len b (len - 1);
@@ -109,7 +126,7 @@ let rec bn_v_is_nat_from_intseq_le_lemma len b =
 val bn_from_bytes_be_lemma_: len:size_nat{8 * len <= max_size_t} -> b:lseq uint8 (8 * len) -> Lemma
   (bn_v (bn_from_bytes_be_ len b) == nat_from_bytes_be b)
 let bn_from_bytes_be_lemma_ len b =
-  bn_v_is_nat_from_intseq_le_lemma len (bn_from_bytes_be_ len b);
+  bn_v_is_nat_from_intseq_be_lemma len (bn_from_bytes_be_ len b);
   bn_from_bytes_be_is_uints_from_bytes_be_reverse len b;
   twice_reverse (uints_from_bytes_be #U64 #SEC #len b);
   assert (bn_v (bn_from_bytes_be_ len b) == nat_from_intseq_be (uints_from_bytes_be #U64 #SEC #len b));
@@ -231,3 +248,99 @@ let bn_to_bytes_be_lemma len b =
 
   Classical.forall_intro lemma_aux;
   eq_intro (nat_to_intseq_be #U8 #SEC len (bn_v b)) res
+
+
+(* Little-endian *)
+
+val bn_v_is_nat_from_intseq_le_lemma: len:size_nat -> b:lseq uint64 len -> Lemma (bn_v b == nat_from_intseq_le b)
+let rec bn_v_is_nat_from_intseq_le_lemma len b =
+  if len = 0 then
+    bn_eval0 b
+  else begin
+    let b1 = slice b 0 (len - 1) in
+    bn_v_is_nat_from_intseq_le_lemma (len - 1) b1;
+    assert (bn_v b1 == nat_from_intseq_le b1);
+
+    bn_eval_split_i #len b (len - 1);
+    //assert (bn_v b == bn_v b1 + pow2 (64 * (len - 1)) * bn_v (slice b (len - 1) len));
+    bn_eval_unfold_i #1 (slice b (len - 1) len) 1;
+    bn_eval0 #1 (slice b (len - 1) len);
+    //assert (bn_v (slice b (len - 1) len) == v b.[len - 1]);
+    assert (bn_v b == nat_from_intseq_le b1 + pow2 (64 * (len - 1)) * v b.[len - 1]);
+    nat_from_intseq_le_slice_lemma b (len - 1);
+    //assert (nat_from_intseq_le b == nat_from_intseq_le b1 + pow2 ((len - 1) * 64) * nat_from_intseq_le (slice b (len - 1) len));
+    nat_from_intseq_le_lemma0 (slice b (len - 1) len);
+    assert (nat_from_intseq_le b == nat_from_intseq_le b1 + pow2 ((len - 1) * 64) * v b.[len - 1]) end
+
+
+val lemma_nat_from_bytes_le_zeroes: len:size_nat -> b:lseq uint8 len -> Lemma
+  (requires (forall (i:nat). i < len ==> b.[i] == u8 0))
+  (ensures  nat_from_intseq_le b == 0)
+
+let rec lemma_nat_from_bytes_le_zeroes len b =
+  if len = 0 then ()
+  else begin
+    nat_from_intseq_le_slice_lemma #U8 #SEC #len b 1;
+    nat_from_intseq_le_lemma0 (slice b 0 1);
+    lemma_nat_from_bytes_le_zeroes (len-1) (slice b 1 len) end
+
+
+val nat_from_bytes_le_eq_lemma: len0:size_nat -> len:size_nat{len0 <= len} -> b:lseq uint8 len0 -> Lemma
+ (let tmp = create len (u8 0) in
+  nat_from_intseq_le b == nat_from_intseq_le (update_sub tmp 0 len0 b))
+
+let nat_from_bytes_le_eq_lemma len0 len b =
+  let tmp = create len (u8 0) in
+  let r = update_sub tmp 0 len0 b in
+  assert (slice r 0 len0 == b);
+  assert (forall (i:nat). i < len - len0 ==> r.[len0 + i] == u8 0);
+  nat_from_intseq_le_slice_lemma #U8 #SEC #len r len0;
+  assert (nat_from_intseq_le r == nat_from_intseq_le (slice r 0 len0) + pow2 (len0 * 8) * nat_from_intseq_le (Seq.slice r len0 len));
+  assert (nat_from_intseq_le r == nat_from_intseq_le b + pow2 (len0 * 8) * nat_from_intseq_le (Seq.slice r len0 len));
+  lemma_nat_from_bytes_le_zeroes (len - len0) (Seq.slice r len0 len)
+
+
+val bn_from_bytes_le_lemma: len:size_pos{8 * (blocks len 8) <= max_size_t} -> b:lseq uint8 len ->
+  Lemma (bn_v (bn_from_bytes_le len b) == nat_from_bytes_le b)
+let bn_from_bytes_le_lemma len b =
+  let bnLen = blocks len 8 in
+  let tmpLen = 8 * bnLen in
+  let tmp = create tmpLen (u8 0) in
+  let tmp = update_sub tmp 0 len b in
+  let res = uints_from_bytes_le #U64 #SEC #bnLen tmp in
+  uints_from_bytes_le_nat_lemma #U64 #SEC #bnLen tmp;
+  //assert (nat_from_intseq_le res == nat_from_intseq_le tmp);
+  bn_v_is_nat_from_intseq_le_lemma bnLen res;
+  //assert (bn_v res == nat_from_intseq_le res);
+  nat_from_bytes_le_eq_lemma len tmpLen b
+  //assert (nat_from_intseq_le tmp == nat_from_intseq_le b)
+
+
+val bn_to_bytes_le_lemma:
+    len:size_pos{8 * (blocks len 8) <= max_size_t}
+  -> b:lbignum (blocks len 8){bn_v b < pow2 (8 * len)} ->
+  Lemma (bn_to_bytes_le len b == nat_to_intseq_le #U8 len (bn_v b))
+let bn_to_bytes_le_lemma len b =
+  let bnLen = blocks len 8 in
+  let tmpLen = 8 * bnLen in
+  let tmp = uints_to_bytes_le b in
+  let res = sub tmp 0 len in
+  assert (bn_v b < pow2 (8 * len));
+  Math.Lemmas.pow2_le_compat (64 * bnLen) (8 * len);
+  assert (bn_v b < pow2 (64 * bnLen));
+
+  uints_to_bytes_le_nat_lemma #U64 #SEC bnLen (bn_v b);
+  //assert (uints_to_bytes_le #U64 #SEC #bnLen (nat_to_intseq_le #U64 #SEC bnLen (bn_v b)) == nat_to_bytes_le (bnLen * 8) (bn_v b));
+  bn_v_is_nat_from_intseq_le_lemma bnLen b;
+  lemma_nat_from_to_intseq_le_preserves_value bnLen b;
+  //assert (nat_to_intseq_le #U64 #SEC bnLen (bn_v b) == b);
+  assert (uints_to_bytes_le #U64 #SEC #bnLen b == nat_to_intseq_le #U8 (bnLen * 8) (bn_v b));
+
+  let aux (i:nat{i < len}) :
+    Lemma (index #uint8 #tmpLen (nat_to_intseq_le #U8 (bnLen * 8) (bn_v b)) i ==
+           index #uint8 #len (nat_to_intseq_le #U8 len (bn_v b)) i) =
+    index_nat_to_intseq_le #U8 #SEC (bnLen * 8) (bn_v b) i;
+    index_nat_to_intseq_le #U8 #SEC len (bn_v b) i in
+
+  Classical.forall_intro aux;
+  eq_intro (nat_to_intseq_le #U8 #SEC len (bn_v b)) res
